4) Six math books, four physics books, and three chemistry books are arranged on a shelf. How many arrangements are possible if all books of the same subject are grouped together
## 5) How many 4-permutations are there of the set \{A,B,C,D,E,F\} if whenever A appears in the permutation, it is followed by E?

We can break this problem up into 2 disjoint cases and then apply the addition principle to get the total number of possibilities. 

**Case 1:** Choose 4 items from the set without A.
This reduced set has a length of 5. This is equivalent to doing $P(n=5, k=4)$ which is the number of different ways to arrange 4 items from a set of 5. 

So $5 \cdot 4 \cdot 3 \cdot 2=120$.

**Case 2:** Choose 4 items and apply the "A follows E" rule.
1. Determine the number of ways to arrange A and E
A can only go in the first 3 spots (_ _ _ ) _ because there has to be space to fit an E after the occurence of an A. 

There are 3 different ways to put A and E in these three spots
A E _ _ ,  _ A E _  , _ _ A E 

2. Determine the number of ways to pick the remaining spots
For each of those 3 ways, we have 2 letters remaining. Since we have already picked 2 letters from the set (A and E), there are 4 letters remaining to choose from.

Therefore, there are 4 choices for the first letter and 3 choices for the second
$4 * 3 = 12$

3. Count the total number of possibilities
For case 1, there are a total of 120 different arrangements.

Since there are 3 different ways to arrange AE together and each of those ways have 12 ways to "fill in the blanks", there are a total of 36 options for case 2.

Therefore, the total is 156 4-permutations. 

# 16) The indicated diagonals of Pascal's triangle sum to the Fibonacci Numbers. Prove this pattern continues forever.
https://ximera.osu.edu/math/combinatorics/combinatoricsBook/combinatoricsBook/combinatorics/identities/identities

It appears that if you sum along the diagonal's of Pascal's triangle, it follow's the Fibonacci sequence. Pascal's triangle is often used to find the coefficients of a binomial $(x+y)^{n}$. This can also be expressed with combinatorics, which is written on the side of each bubble in the triangle. 

For this post we will assume that $F_{0}=1$, $F_{1}=1$ and the Fibonacci sequence is generated by $F_{n}=F_{n-1}+F_{n-2}$.

To demonstrate this using combinatorics, the 4th (5th if you don't count from 0) diagonal's sum looks like
$$
{4 \choose 0} + {3 \choose 1} + {2 \choose 2} =1+3+1 = 5
$$
Which is equal to $F_{4}$ . 

We can extrapolate and guess that the pattern continues along the lines of $F_{n} =\sum_{k=0}{n -k \choose k }$. The top term, $n-k$, decreases as k increase, while the bottom number $k$ increases with the sum.

However the number of terms in a diagonal depends on the particular Fibonacci number you are evaluating. If you look at the table in the photo, the number of terms in a diagonal follows a floor pattern. The expression is exactly $\lfloor \frac{n}{2}+1 \rfloor$

![[Pasted image 20230407162409.png]]

We will prove with strong induction that the n-th Fibonacci number is equal to
$$
F_{n}=\sum_{k=0}^{\lfloor \frac{n}{2} +1\rfloor } {n-k \choose k}
$$

# Proof
### Base case
When $n=0$, $F_{n}=1$ and $\sum_{k=0}^{\lfloor 0+1 \rfloor}{0-k \choose k}={0-0 \choose 0}+{0-1 \choose 0}=1+0=1$. Which are equal.
When $n=1$, $F_{n}=1$ and $\sum_{k=0}^{\lfloor \frac{1}{2}+1 \rfloor}{1-k \choose k }={1-0 \choose 0}+{1-1 \choose 1}=1+0=1$.  Which are equal.

Therefore, the base case holds.

### Inductive step
Assume that for $j\in\mathbb{N}$ and $j\geq 1$ we know how to construct the k-th Fibonacci number as long as it is in the interval $0 \leq k \leq j$ (the interval our base cases are in). 

Consider the $j+1$ Fibonacci number. We will proceed with a proof by cases, when $j$ is even and when $j$ is odd. 

#### Case 1: $j$ is even.
Because $j$ is even, it is a multiple of two. So $j=2m$, $m \in \mathbb{Z}$. Then we know that 
$$
F_{j}=\sum_{k=0}^{\lfloor \frac{2m}{2}+1 \rfloor} {j-k \choose k} \text{ and }F_{j-1}=\sum_{k=0}^{\lfloor \frac{2m-1}{2}+1 \rfloor} {j-k \choose k}
$$We can simplify the upper bounds of each sum. 

For $F_{j}$, $\lfloor \frac{j}{2}+1 \rfloor=\lfloor \frac{2m}{2}+1 \rfloor=\lfloor m+1 \rfloor=m+1$ 
For $F_{j-1}$, $\lfloor \frac{j-1}{2}+1 \rfloor=\lfloor \frac{2m-1}{2}+1 \rfloor=\lfloor m+\frac{1}{2} \rfloor=m$

Therefore $F_{j}=\sum_{k=0}^{m+1}{2m-k \choose k}$ and $F_{j-1}=\sum_{k=0}^{m}{2m-1-k \choose k}$

Continuing with the proof, we will make use of the fact that ${n \choose k-1}+{n \choose k}={n+1 \choose k}$ ([See proof](https://ximera.osu.edu/math/combinatorics/combinatoricsBook/combinatoricsBook/combinatorics/identities/identities))

$$
\begin{align}
F_{j+1}=\sum_{k=0}^{m+1}{(2m+1)-k \choose k} = \sum_{k=0}^{m+1}{2m-k \choose k}+\sum_{k=0}^{m+1}{2m-k \choose k-1} \\
=F_{j}+\sum_{k=0}^{m+1}{2m-k \choose k-1}  \\
=F_{j}+\cancel{2m-0 \choose 0-1}+\sum_{k=1}^{m+1}{2m-k \choose k-1} \\
\end{align}
$$
We evaluate the first term of the sum. This ends up being 0 because you can't choose a negative number of elements (0 ways to do so) ${2m-0 \choose 0-1}={2m \choose -1}=0$. Next we re-index the sum. Let $u=k-1$, then
$$
\begin{align}
F_{j+1}=F_{j}+\sum_{u=0}^{m}{2m-(u+1) \choose u} \\
F_{j+1}=F_{j}+\sum_{u=0}^{m}{2m-1-u \choose u} \\
F_{j+1}=F_{j}+F_{j-1}
\end{align}
$$

#### Case 2: $j$ is odd.
Because $j$ is odd, then it can be written as a multiple of 2 plus one. So $j=2m+1$ where $m \in\mathbb{Z}$. 

To streamline our work, let us simplify the floor evaluations.
For $j$, $\lfloor \frac{j}{2}+1 \rfloor=\lfloor \frac{2m+1}{2}+1 \rfloor=\lfloor m+\frac{3}{2} \rfloor=m+1$
For $j+1$, $\lfloor \frac{j+1}{2} +1 \rfloor = \lfloor \frac{2m+1+1}{2}+1 \rfloor=\lfloor m+2 \rfloor=m+2$
For $j-1$, $\lfloor \frac{j-1}{2}+1 \rfloor = \lfloor \frac{2m+1-1}{2}+1 \rfloor=\lfloor m+1 \rfloor=m+1$

Then $F_{j}=\sum_{k=0}^{m+1}{(2m+1)-k \choose k}$ and $F_{j-1}=\sum_{k=0}^{m+1}{2m-k \choose k}$.

Continuing with the proof and making use of the same identity as before:
$$
\begin{align}
F_{j+1}=\sum_{k=0}^{m+2}{(2m+1)+1-k \choose k } = \sum_{k=0}^{m+2}{(2m+1-k)+1 \choose k } \\
=\sum_{k=0}^{m+2}{2m+1-k \choose k}+\sum_{k=0}^{m+2}{2m+1-k \choose k-1}
\end{align}
$$
We evaluate the **last** term of the first sum. Then we evaluate the **first** term of the second sum.
$$
\begin{align}
F_{j+1}={2m+1 - (m+2) \choose m+2 } +\sum_{k=0}^{m+1}{2m+1-k \choose k}+{2m+1-0 \choose 0-1}+\sum_{k=0}^{m+2}{2m+1-k \choose k-1} \\
=\cancel{m-1 \choose m+2 } +F_{j}+ \cancel{2m+1 \choose -1}+\sum_{k=1}^{m+2}{2m+1-k \choose k-1}
\end{align}
$$
Re-index the second sum. Let $u=k-1$.
$$
\begin{align}
F_{j+1}=F_{j}+\sum_{u=0}^{m+1}{2m+1-(u+1) \choose u} \\
= F_{j}+\sum_{u=0}^{m+1}{2m-u \choose u}=F_{j}+F_{j-1}
\end{align}
$$

$\therefore$ Therefore, we have shown using strong induction that the sum along the diagonals of Pascal's triangle follow's the Fibonacci sequence. 

